Finish stlc example.

coq/theories/Examples/stlc_new.v
@@ -118,6 +118,9 @@ with v_subst {Γ Δ} : Γ =[val]> Δ -> val Γ ⇒ᵢ val Δ :=
 Equations s_subst {Γ Δ} : Γ =[val]> Δ -> state Γ -> state Δ :=
   s_subst f (Cut v k) := Cut (t_subst f _ v) (v_subst f _ k).
 
+Definition a_comp {Γ1 Γ2 Γ3} : Γ2 =[val]> Γ3 -> Γ1 =[val]> Γ2 -> Γ1 =[val]> Γ3 :=
+  fun f g _ i => v_subst f _ (g _ i) .
+
 (* Substitution of a single variable and of a pair of variables *)
 Definition ass1 {Γ a} (v : val Γ a) : (Γ ▶ a) =[val]> Γ := s_append a_id v .
 Definition t_subst1  {Γ a b} (u : term (Γ ▶ a) b) v := t_subst (ass1 v) _ u.
@@ -145,16 +148,17 @@ Notation "u /ₜ[ v , w ]" := (t_subst2 u v w) (at level 50, left associativity)
    so degenerate that we omit the following definitions and simply inline them.
    In contrast, compare with the situation for [MuMuTilde] that features in particular
    positive types.
+PB: TODO fix comment
+*)
 
- Open Scope ctx_scope.
- Definition pat : ty -> Type := fun _ => unit.
- Definition pat_dom {a} : pat a -> t_ctx := fun _ => ∅ ▶ a.
- Definition v_of_p {a} (p : pat a) : val (pat_dom p) a := Var top.
- Definition p_of_v {Γ : t_ctx} a : val Γ a -> pat a := fun _ => tt.
- Definition p_dom_of_v {Γ : t_ctx} a (v : val Γ a) : pat_dom (p_of_v a v) =[val]> Γ
-   := s_append s_empty v.
+Variant pat : ty -> Type :=
+| PPos {a} : pat (t+ a)
+| PApp {a b} : pat (t- (a → b))
+.
 
- *)
+Equations pat_dom {a} : pat a -> t_ctx :=
+  pat_dom (@PPos a)   := ∅ ▶ t+ a ;
+  pat_dom (@PApp a b) := ∅ ▶ t+ a ▶ t- b .
 
 (** * Normal forms
     Normal forms happen when stuck on a variable [x] of some type [a].
@@ -163,9 +167,9 @@ Notation "u /ₜ[ v , w ]" := (t_subst2 u v w) (at level 50, left associativity)
     - for a producer type: "⟨ x | π ⟩"
     - for a consumer type: "⟨ v | x ⟩"
  *)
-Definition nf0 (Γ : t_ctx) (a : ty) : Type := val Γ (t_neg a).
+Definition nf0 (Γ : t_ctx) (a : ty) : Type := { p : pat a & pat_dom p =[val]> Γ } .
 Definition nf  (Γ : t_ctx) : Type :=
-  { a : ty & (Γ ∋ a * nf0 Γ a)%type } .
+  { a : ty & (Γ ∋ a * nf0 Γ (t_neg a))%type } .
 
 (** * Evaluator
     The (call-by-value) evaluator. The reduction rules should come to no surprise:
@@ -185,21 +189,566 @@ Definition nf  (Γ : t_ctx) : Type :=
     the corresponding normal form.
  *)
 Equations eval_aux {Γ : t_ctx} : state Γ -> (state Γ + nf Γ) :=
-  {
-    eval_aux (Cut (Val v) (KFun t π))          :=
-      inl (Cut t (KArg v π));
-    eval_aux (Cut (Val v) (Var i))             :=
-      inr (t-_ ,' (i,v));
+  eval_aux (Cut (App t1 t2)      (π))        := inl (Cut t2 (KFun t1 π)) ;
+  eval_aux (Cut (Val v)          (Var i))    := inr (_ ,' (i, (PPos ,' s_append s_empty v))) ;
+  eval_aux (Cut (Val v)          (KFun t π)) := inl (Cut t (KArg v π)) ;
+  eval_aux (Cut (Val (Var i))    (KArg v π)) := inr (_,' (i, (PApp ,' (s_append (s_append s_empty v) π)))) ;
+  eval_aux (Cut (Val (LamRec t)) (KArg v π)) := inl (Cut (t/ₜ[ LamRec t , v ]) π) .
 
-    eval_aux (Cut (Val (Var i))    π)          :=
-      inr (t+_,' (i,π));
-
-    eval_aux (Cut (Val (LamRec t)) (KArg v π)) :=
-      inl (Cut (t/ₜ[LamRec t , v]) π);
-
-    eval_aux (Cut (App t1 t2)    π)            :=
-      inl (Cut t2 (KFun t1 π))
-  }.
 Definition eval {Γ : t_ctx} : state Γ -> delay (nf Γ)
   := iter_delay (fun c => Ret' (eval_aux c)).
-Notation play := eval.
+
+Definition p_app {Γ x} (v : val Γ x) (m : pat (t_neg x)) (γ : pat_dom m =[val]> Γ) : state Γ .
+  destruct x; cbn in *; dependent elimination m; cbn in *.
+  - exact (Cut (Val v) (KArg (γ _ (pop top)) (γ _ top))).
+  - exact (Cut (Val (γ _ top)) v).
+Defined.
+
+Scheme term_mut := Induction for term Sort Prop
+   with val_mut := Induction for val Sort Prop .
+
+Record syn_ind_args (P_t : forall Γ A, term Γ A -> Prop)
+                    (P_v : forall Γ A, val Γ A -> Prop) :=
+  {
+    ind_s_val {Γ a} v (_ : P_v Γ a v) : P_t Γ a (Val v) ;
+    ind_s_app {Γ a b} t1 (_ : P_t Γ (t+ (a → b)) t1) t2 (_ : P_t Γ (t+ a) t2) : P_t Γ (t+ b) (App t1 t2) ;
+    ind_s_var {Γ a} i : P_v Γ a (Var i) ;
+    ind_s_lamrec {Γ a b} t (_ : P_t (Γ ▶ t+ (a → b) ▶ t+ a)%ctx (t+ b) t) : P_v Γ (t+ (a → b)) (LamRec t) ;
+    ind_s_kfun {Γ a b} t (_ : P_t Γ (t+ (a → b)) t) π (_ : P_v Γ (t- b) π) : P_v Γ (t- a) (KFun t π) ;
+    ind_s_karg {Γ a b} v (_ : P_v Γ (t+ a) v) π (_ : P_v Γ (t- b) π) : P_v Γ (t- (a → b)) (KArg v π) ;
+  } .
+
+Lemma term_ind_mut P_t P_v (H : syn_ind_args P_t P_v) Γ a t : P_t Γ a t .
+  destruct H; now apply (term_mut P_t P_v).
+Qed.
+
+Lemma val_ind_mut P_t P_v (H : syn_ind_args P_t P_v) Γ a v : P_v Γ a v .
+  destruct H; now apply (val_mut P_t P_v).
+Qed.
+
+Definition t_ren_proper_P Γ a (t : term Γ a) : Prop :=
+  forall Δ (f1 f2 : Γ ⊆ Δ), f1 ≡ₐ f2 -> t_rename f1 a t = t_rename f2 a t .
+Definition v_ren_proper_P Γ a (v : val Γ a) : Prop :=
+  forall Δ (f1 f2 : Γ ⊆ Δ), f1 ≡ₐ f2 -> v_rename f1 a v = v_rename f2 a v .
+Lemma ren_proper_prf : syn_ind_args t_ren_proper_P v_ren_proper_P.
+  econstructor.
+  all: unfold t_ren_proper_P, v_ren_proper_P.
+  all: intros; cbn; f_equal; auto.
+  now apply H.
+  now apply H, r_shift_eq, r_shift_eq.
+Qed.
+
+#[global] Instance t_ren_eq {Γ Δ}
+  : Proper (ass_eq _ _ ==> forall_relation (fun a => eq ==> eq)) (@t_rename Γ Δ).
+  intros f1 f2 H1 a x y ->; now apply (term_ind_mut _ _ ren_proper_prf).
+Qed.
+
+#[global] Instance v_ren_eq {Γ Δ}
+  : Proper (ass_eq _ _ ==> forall_relation (fun a => eq ==> eq)) (@v_rename Γ Δ).
+  intros f1 f2 H1 a x y ->; now apply (val_ind_mut _ _ ren_proper_prf).
+Qed.
+
+#[global] Instance s_ren_eq {Γ Δ}
+  : Proper (ass_eq _ _ ==> eq ==> eq) (@s_rename Γ Δ).
+  intros f1 f2 H1 x y ->; destruct y; cbn; now rewrite H1.
+Qed.
+
+#[global] Instance a_ren_eq {Γ1 Γ2 Γ3}
+  : Proper (ass_eq _ _ ==> ass_eq _ _ ==> ass_eq _ _) (@a_ren Γ1 Γ2 Γ3).
+  intros r1 r2 H1 a1 a2 H2 ? i; unfold a_ren; cbn.
+  apply (v_ren_eq _ _ H1), H2.
+Qed.
+
+#[global] Instance a_shift_eq {Γ Δ y} : Proper (ass_eq _ _ ==> ass_eq _ _) (@a_shift Γ Δ y).
+  intros ? ? H ? h.
+  dependent elimination h; cbn; auto.
+  now rewrite H.
+Qed.
+
+#[global] Instance a_shift2_eq {Γ Δ x y} : Proper (ass_eq _ _ ==> ass_eq _ _) (@a_shift2 Γ Δ x y).
+  intros ? ? H ? h.
+  do 2 (dependent elimination h; cbn; auto).
+  now rewrite H.
+Qed.
+
+Definition t_ren_ren_P Γ1 a (t : term Γ1 a) : Prop :=
+  forall Γ2 Γ3 (f1 : Γ2 ⊆ Γ3) (f2 : Γ1 ⊆ Γ2),
+    t_rename f1 a (t_rename f2 a t) = t_rename (s_ren f1 f2) a t.
+Definition v_ren_ren_P Γ1 a (v : val Γ1 a) : Prop :=
+  forall Γ2 Γ3 (f1 : Γ2 ⊆ Γ3) (f2 : Γ1 ⊆ Γ2),
+    v_rename f1 a (v_rename f2 a v) = v_rename (s_ren f1 f2) a v.
+
+Lemma ren_ren_prf : syn_ind_args t_ren_ren_P v_ren_ren_P.
+  econstructor.
+  all: unfold t_ren_ren_P, v_ren_ren_P.
+  all: intros; cbn; f_equal; auto.
+  all: unfold r_shift2; now repeat rewrite r_shift_comp.
+Qed.
+
+Lemma t_ren_ren {Γ1 Γ2 Γ3} (f1 : Γ2 ⊆ Γ3) (f2 : Γ1 ⊆ Γ2) a (t : term Γ1 a)
+  : t_rename f1 a (t_rename f2 a t) = t_rename (s_ren f1 f2) a t.
+  now apply (term_ind_mut _ _ ren_ren_prf).
+Qed.
+Lemma v_ren_ren {Γ1 Γ2 Γ3} (f1 : Γ2 ⊆ Γ3) (f2 : Γ1 ⊆ Γ2) a (v : val Γ1 a)
+  : v_rename f1 a (v_rename f2 a v) = v_rename (s_ren f1 f2) a v.
+  now apply (val_ind_mut _ _ ren_ren_prf).
+Qed.
+Lemma s_ren_ren {Γ1 Γ2 Γ3} (f1 : Γ2 ⊆ Γ3) (f2 : Γ1 ⊆ Γ2) (s : state Γ1)
+  : s_rename f1 (s_rename f2 s) = s_rename (s_ren f1 f2) s.
+  destruct s; cbn; f_equal.
+  now apply t_ren_ren.
+  now apply v_ren_ren.
+Qed.
+
+Definition t_ren_id_l_P Γ a (t : term Γ a) : Prop := t_rename r_id a t = t.
+Definition v_ren_id_l_P Γ a (v : val Γ a)  : Prop := v_rename r_id a v = v.
+
+Lemma ren_id_l_prf : syn_ind_args t_ren_id_l_P v_ren_id_l_P.
+  econstructor.
+  all: unfold t_ren_id_l_P, v_ren_id_l_P.
+  all: intros; cbn; f_equal; auto.
+  unfold r_shift2; now repeat rewrite r_shift_id.
+Qed.
+
+Lemma t_ren_id_l {Γ} a (t : term Γ a) : t_rename r_id a t = t.
+  now apply (term_ind_mut _ _ ren_id_l_prf).
+Qed.
+Lemma v_ren_id_l {Γ} a (v : val Γ a) : v_rename r_id a v = v.
+  now apply (val_ind_mut _ _ ren_id_l_prf).
+Qed.
+Lemma s_ren_id_l {Γ} (s : state Γ) : s_rename r_id s = s.
+  destruct s; cbn; f_equal.
+  now apply t_ren_id_l.
+  now apply v_ren_id_l.
+Qed.
+
+Lemma v_ren_id_r {Γ Δ} (f : Γ ⊆ Δ) a (i : Γ ∋ a) : v_rename f a (Var i) = Var (f _ i).
+  reflexivity.
+Qed.
+
+Lemma a_shift_id {Γ a} : @a_shift Γ Γ a a_id ≡ₐ a_id.
+  intros x i; destruct x; dependent elimination i; auto.
+Qed.
+
+Lemma a_shift2_id {Γ x y} : @a_shift2 Γ Γ x y a_id ≡ₐ a_id.
+  unfold a_shift2, v_shift2; intros ? h.
+  do 2 (dependent elimination h; cbn; auto).
+Qed.
+
+Lemma a_shift_a_ren {Γ1 Γ2 Γ3 y} (f1 : Γ2 ⊆ Γ3) (f2 : Γ1 =[ val ]> Γ2)
+      : a_shift (y:=y) (a_ren f1 f2) ≡ₐ a_ren (r_shift f1) (a_shift f2) .
+  unfold r_shift, a_shift, a_ren, v_shift; intros ? h.
+  dependent elimination h; cbn; auto.
+  now rewrite 2 v_ren_ren.
+Qed.
+
+Lemma a_shift_s_ren {Γ1 Γ2 Γ3 y} (f1 : Γ2 =[val]> Γ3) (f2 : Γ1 ⊆ Γ2)
+  : a_shift (y:=y) (s_ren f1 f2) ≡ₐ s_ren (a_shift f1) (r_shift f2) .
+  intros ? i; dependent elimination i; auto.
+Qed.
+
+Lemma a_shift2_s_ren {Γ1 Γ2 Γ3 x y} (f1 : Γ2 =[val]> Γ3) (f2 : Γ1 ⊆ Γ2)
+  : a_shift2 (x:=x) (y:=y) (s_ren f1 f2) ≡ₐ s_ren (a_shift2 f1) (r_shift2 f2) .
+  intros ? h; do 2 (dependent elimination h; auto).
+Qed.
+
+Lemma a_shift2_a_ren {Γ1 Γ2 Γ3 x y} (f1 : Γ2 ⊆ Γ3) (f2 : Γ1 =[ val ]> Γ2)
+      : a_shift2 (x:=x) (y:=y) (a_ren f1 f2) ≡ₐ a_ren (r_shift2 f1) (a_shift2 f2) .
+  unfold r_shift2, r_shift, a_shift2, v_shift2, a_ren; intros ? h.
+  do 2 (dependent elimination h; cbn; auto).
+  now rewrite 2 v_ren_ren.
+Qed.
+
+Definition t_sub_proper_P Γ a (t : term Γ a) : Prop :=
+  forall Δ (f1 f2 : Γ =[val]> Δ), f1 ≡ₐ f2 -> t_subst f1 a t = t_subst f2 a t .
+Definition v_sub_proper_P Γ a (v : val Γ a) : Prop :=
+  forall Δ (f1 f2 : Γ =[val]> Δ), f1 ≡ₐ f2 -> v_subst f1 a v = v_subst f2 a v .
+
+Lemma sub_proper_prf : syn_ind_args t_sub_proper_P v_sub_proper_P.
+  econstructor.
+  all: unfold t_sub_proper_P, v_sub_proper_P.
+  all: intros; cbn; f_equal; auto.
+  now apply H, a_shift2_eq.
+Qed.
+
+#[global] Instance t_sub_eq {Γ Δ}
+  : Proper (ass_eq _ _ ==> dpointwise_relation (fun a => eq ==> eq)) (@t_subst Γ Δ).
+  intros f1 f2 H1 a x y ->; now apply (term_ind_mut _ _ sub_proper_prf).
+Qed.
+
+#[global] Instance v_sub_eq {Γ Δ}
+  : Proper (ass_eq _ _ ==> dpointwise_relation (fun a => eq ==> eq)) (@v_subst Γ Δ).
+  intros f1 f2 H1 a x y ->; now apply (val_ind_mut _ _ sub_proper_prf).
+Qed.
+
+#[global] Instance s_sub_eq {Γ Δ}
+  : Proper (ass_eq _ _ ==> eq ==> eq) (@s_subst Γ Δ).
+  intros f1 f2 H1 x y ->; destruct y; cbn; f_equal.
+  now apply t_sub_eq.
+  now apply v_sub_eq.
+Qed.
+
+#[global] Instance a_comp_eq {Γ1 Γ2 Γ3} : Proper (ass_eq _ _ ==> ass_eq _ _ ==> ass_eq _ _) (@a_comp Γ1 Γ2 Γ3).
+  intros ? ? H1 ? ? H2 ? ?; apply v_sub_eq; [ apply H1 | apply H2 ].
+Qed.
+
+Definition t_ren_sub_P Γ1 a (t : term Γ1 a) : Prop :=
+  forall Γ2 Γ3 (f1 : Γ2 ⊆ Γ3) (f2 : Γ1 =[val]> Γ2),
+    t_rename f1 a (t_subst f2 a t)
+    = t_subst (a_ren f1 f2) a t .
+Definition v_ren_sub_P Γ1 a (v : val Γ1 a) : Prop :=
+  forall Γ2 Γ3 (f1 : Γ2 ⊆ Γ3) (f2 : Γ1 =[val]> Γ2),
+    v_rename f1 a (v_subst f2 a v)
+    = v_subst (a_ren f1 f2) a v .
+Lemma ren_sub_prf : syn_ind_args t_ren_sub_P v_ren_sub_P.
+  econstructor.
+  all: unfold t_ren_sub_P, v_ren_sub_P.
+  all: intros; cbn; f_equal; auto.
+  etransitivity; [ now apply H | ].  
+  eapply t_sub_eq; auto.
+  symmetry; apply a_shift2_a_ren.
+Qed.
+Lemma t_ren_sub {Γ1 Γ2 Γ3} (f1 : Γ2 ⊆ Γ3) (f2 : Γ1 =[val]> Γ2) a (t : term Γ1 a)
+  : t_rename f1 a (t_subst f2 a t) = t_subst (a_ren f1 f2) a t.
+  now apply (term_ind_mut _ _ ren_sub_prf).
+Qed.
+Lemma v_ren_sub {Γ1 Γ2 Γ3} (f1 : Γ2 ⊆ Γ3) (f2 : Γ1 =[val]> Γ2) a (v : val Γ1 a)
+  : v_rename f1 a (v_subst f2 a v) = v_subst (a_ren f1 f2) a v.
+  now apply (val_ind_mut _ _ ren_sub_prf).
+Qed.
+Lemma s_ren_sub {Γ1 Γ2 Γ3} (f1 : Γ2 ⊆ Γ3) (f2 : Γ1 =[val]> Γ2) (s : state Γ1)
+  : s_rename f1 (s_subst f2 s) = s_subst (a_ren f1 f2) s.
+  destruct s; cbn; f_equal.
+  now apply t_ren_sub.
+  now apply v_ren_sub.
+Qed.
+
+Definition t_sub_ren_P Γ1 a (t : term Γ1 a) : Prop :=
+  forall Γ2 Γ3 (f1 : Γ2 =[val]> Γ3) (f2 : Γ1 ⊆ Γ2),
+    t_subst f1 a (t_rename f2 a t)
+    = t_subst (s_ren f1 f2) a t .
+Definition v_sub_ren_P Γ1 a (v : val Γ1 a) : Prop :=
+  forall Γ2 Γ3 (f1 : Γ2 =[val]> Γ3) (f2 : Γ1 ⊆ Γ2),
+    v_subst f1 a (v_rename f2 a v)
+    = v_subst (s_ren f1 f2) a v .
+Lemma sub_ren_prf : syn_ind_args t_sub_ren_P v_sub_ren_P.
+  econstructor.
+  all: unfold t_sub_ren_P, v_sub_ren_P.
+  all: intros; cbn; f_equal; auto.
+  etransitivity; [ now apply H | ].  
+  eapply t_sub_eq; auto.
+  symmetry; apply a_shift2_s_ren.
+Qed.
+
+Lemma t_sub_ren {Γ1 Γ2 Γ3} (f1 : Γ2 =[val]> Γ3) (f2 : Γ1 ⊆ Γ2) a (t : term Γ1 a)
+  : t_subst f1 a (t_rename f2 a t) = t_subst (s_ren f1 f2) a t.
+  now apply (term_ind_mut _ _ sub_ren_prf).
+Qed.
+Lemma v_sub_ren {Γ1 Γ2 Γ3} (f1 : Γ2 =[val]> Γ3) (f2 : Γ1 ⊆ Γ2) a (v : val Γ1 a)
+  : v_subst f1 a (v_rename f2 a v) = v_subst (s_ren f1 f2) a v.
+  now apply (val_ind_mut _ _ sub_ren_prf).
+Qed.
+Lemma s_sub_ren {Γ1 Γ2 Γ3} (f1 : Γ2 =[val]> Γ3) (f2 : Γ1 ⊆ Γ2) (s : state Γ1)
+  : s_subst f1 (s_rename f2 s) = s_subst (s_ren f1 f2) s.
+  destruct s; cbn; f_equal.
+  now apply t_sub_ren.
+  now apply v_sub_ren.
+Qed.
+
+Lemma v_sub_id_r {Γ Δ} (f : Γ =[val]> Δ) a (i : Γ ∋ a) : v_subst f a (Var i) = f _ i.
+  reflexivity.
+Qed.
+Lemma a_comp_id_r {Γ1 Γ2} (a : Γ1 =[val]> Γ2) : a_comp a a_id ≡ₐ a .
+  intros ? i; auto.
+Qed.
+
+Lemma a_shift_comp {Γ1 Γ2 Γ3 y} (f1 : Γ2 =[val]> Γ3) (f2 : Γ1 =[val]> Γ2)
+  : a_shift (y:=y) (a_comp f1 f2) ≡ₐ a_comp (a_shift f1) (a_shift f2) .
+  intros x i; dependent elimination i; unfold a_shift, a_comp, v_shift; cbn; auto.
+  now rewrite v_ren_sub, v_sub_ren.
+Qed.
+
+Lemma a_shift2_comp {Γ1 Γ2 Γ3 x y} (f1 : Γ2 =[val]> Γ3) (f2 : Γ1 =[val]> Γ2)
+  : a_shift2 (x:=x) (y:=y) (a_comp f1 f2) ≡ₐ a_comp (a_shift2 f1) (a_shift2 f2) .
+  unfold a_shift2, v_shift2, a_comp; intros ? h.
+  do 2 (dependent elimination h; cbn; auto).
+  now rewrite v_ren_sub, v_sub_ren.
+Qed.
+
+Definition t_sub_sub_P Γ1 a (t : term Γ1 a) : Prop :=
+  forall Γ2 Γ3 (f1 : Γ2 =[val]> Γ3) (f2 : Γ1 =[val]> Γ2),
+    t_subst f1 a (t_subst f2 a t) = t_subst (a_comp f1 f2) a t.
+Definition v_sub_sub_P Γ1 a (v : val Γ1 a) : Prop :=
+  forall Γ2 Γ3 (f1 : Γ2 =[val]> Γ3) (f2 : Γ1 =[val]> Γ2),
+    v_subst f1 a (v_subst f2 a v) = v_subst (a_comp f1 f2) a v.
+
+Lemma sub_sub_prf : syn_ind_args t_sub_sub_P v_sub_sub_P.
+  econstructor.
+  all: unfold t_sub_sub_P, v_sub_sub_P.
+  all: intros; cbn; f_equal; auto.
+  etransitivity; [ now apply H | ].
+  apply t_sub_eq; auto.
+  symmetry; apply a_shift2_comp.
+Qed.
+Lemma t_sub_sub {Γ1 Γ2 Γ3} (f1 : Γ2 =[val]> Γ3) (f2 : Γ1 =[val]> Γ2) a (t : term Γ1 a)
+  : t_subst f1 a (t_subst f2 a t) = t_subst (a_comp f1 f2) a t.
+  now apply (term_ind_mut _ _ sub_sub_prf).
+Qed.
+Lemma v_sub_sub {Γ1 Γ2 Γ3} (f1 : Γ2 =[val]> Γ3) (f2 : Γ1 =[val]> Γ2) a (v : val Γ1 a)
+  : v_subst f1 a (v_subst f2 a v) = v_subst (a_comp f1 f2) a v.
+  now apply (val_ind_mut _ _ sub_sub_prf).
+Qed.
+Lemma s_sub_sub {Γ1 Γ2 Γ3} (f1 : Γ2 =[val]> Γ3) (f2 : Γ1 =[val]> Γ2) (s : state Γ1)
+  : s_subst f1 (s_subst f2 s) = s_subst (a_comp f1 f2) s.
+  destruct s; cbn; f_equal.
+  now apply t_sub_sub.
+  now apply v_sub_sub.
+Qed.
+
+Lemma a_comp_assoc {Γ1 Γ2 Γ3 Γ4} (u : Γ3 =[val]> Γ4) (v : Γ2 =[val]> Γ3) (w : Γ1 =[val]> Γ2)
+           : a_comp u (a_comp v w) ≡ₐ a_comp (a_comp u v) w .
+  intros ? i; unfold a_comp; now apply v_sub_sub.
+Qed.
+
+Definition t_sub_id_l_P Γ a (t : term Γ a) : Prop := t_subst a_id a t = t.
+Definition v_sub_id_l_P Γ a (v : val Γ a) : Prop := v_subst a_id a v = v.
+
+Lemma sub_id_l_prf : syn_ind_args t_sub_id_l_P v_sub_id_l_P.
+  econstructor.
+  all: unfold t_sub_id_l_P, v_sub_id_l_P.
+  all: intros; cbn; f_equal; auto.
+  etransitivity; [ | now apply H ].
+  apply t_sub_eq; auto.
+  now apply a_shift2_id.
+Qed.
+
+Lemma t_sub_id_l {Γ} a (t : term Γ a) : t_subst a_id a t = t.
+  now apply (term_ind_mut _ _ sub_id_l_prf).
+Qed.
+Lemma v_sub_id_l {Γ} a (v : val Γ a) : v_subst a_id a v = v.
+  now apply (val_ind_mut _ _ sub_id_l_prf).
+Qed.
+Lemma s_sub_id_l {Γ} (s : state Γ) : s_subst a_id s = s.
+  destruct s; cbn; f_equal.
+  now apply t_sub_id_l.
+  now apply v_sub_id_l.
+Qed.
+Lemma a_comp_id_l {Γ1 Γ2} (a : Γ1 =[val]> Γ2) : a_comp a_id a ≡ₐ a .
+  intros ? i; now apply v_sub_id_l.
+Qed.
+
+
+Lemma sub1_sub {Γ Δ a} (f : Γ =[val]> Δ) (v : val Γ a) :
+  a_comp (ass1 (v_subst f a v)) (a_shift f) ≡ₐ a_comp f (ass1 v).
+  intros ? i; dependent elimination i; cbn; auto.
+  unfold v_shift; rewrite v_sub_ren.
+  now apply v_sub_id_l.
+Qed.
+
+Lemma sub1_ren {Γ Δ a} (f : Γ ⊆ Δ) (v : val Γ a) :
+  ass1 (v_rename f a v) ⊛ᵣ r_shift f ≡ₐ a_ren f (ass1 v) .
+  intros ? i; dependent elimination i; auto.
+Qed.
+
+Lemma v_sub1_sub {Γ Δ a b} (f : Γ =[val]> Δ) (v : val Γ a) (w : val (Γ ▶ a) b)
+  : v_subst (a_shift f) b w /ᵥ v_subst f a v = v_subst f b (w /ᵥ v) .
+  unfold v_subst1; rewrite 2 v_sub_sub.
+  apply v_sub_eq; auto.
+  rewrite sub1_sub; reflexivity.
+Qed.
+
+Lemma v_sub1_ren {Γ Δ a b} (f : Γ ⊆ Δ) (v : val Γ a) (w : val (Γ ▶ a) b)
+  : v_rename (r_shift f) b w /ᵥ v_rename f a v = v_rename f b (w /ᵥ v) .
+  unfold v_subst1. rewrite v_sub_ren, v_ren_sub.
+  apply v_sub_eq; auto.
+  now rewrite sub1_ren.
+Qed.
+
+Lemma t_sub1_sub {Γ Δ a b} (f : Γ =[val]> Δ) (v : val Γ a) (t : term (Γ ▶ a) b)
+  : t_subst (a_shift f) b t /ₜ v_subst f a v = t_subst f b (t /ₜ v) .
+  unfold t_subst1; rewrite 2 t_sub_sub.
+  apply t_sub_eq; auto.
+  rewrite sub1_sub; reflexivity.
+Qed.
+
+Lemma t_sub1_ren {Γ Δ a b} (f : Γ ⊆ Δ) (v : val Γ a) (t : term (Γ ▶ a) b)
+  : t_rename (r_shift f) b t /ₜ v_rename f a v = t_rename f b (t /ₜ v) .
+  unfold t_subst1; rewrite t_sub_ren, t_ren_sub.
+  apply t_sub_eq; auto.
+  now rewrite sub1_ren.
+Qed.
+
+Lemma t_sub2_sub {Γ Δ x y z} (f : Γ =[val]> Δ) (t : term (Γ ▶ x ▶ y) z) u v
+  : t_subst (a_shift2 f) _ t /ₜ[ v_subst f _ u , v_subst f _ v ] = t_subst f _ (t /ₜ[ u , v ]) .
+  unfold t_subst2. rewrite 2 t_sub_sub.
+  apply t_sub_eq; auto.
+  intros ? h; do 2 (dependent elimination h; cbn; auto).
+  unfold v_shift2; rewrite v_sub_ren.
+  now apply v_sub_id_l.
+Qed.
+
+#[global] Instance p_app_eq {Γ x} (v : val Γ x) (m : pat (t_neg x)) : Proper (ass_eq _ _ ==> eq) (p_app v m) .
+  intros u1 u2 H; destruct x; dependent elimination m; cbn in *; do 2 f_equal; apply H.
+Qed.
+
+From OGS.OGS Require Spec.
+
+Definition stlc_spec : Spec.interaction_spec :=
+  {| Spec.typ := ty ;
+     Spec.msg := fun t => pat (t_neg t) ;
+     Spec.dom := fun t p => pat_dom p |}
+.
+
+Program Definition stlc_val : @Spec.lang_monoid stlc_spec :=
+  {| Spec.val := val ;
+     Spec.v_var := @a_id ;
+     Spec.v_sub := @v_subst
+  |}.
+
+Program Definition stlc_conf : @Spec.lang_module stlc_spec stlc_val :=
+  {| Spec.conf := state ;
+     Spec.c_sub := @s_subst ;
+  |}.
+
+Program Definition stlc_val_laws : @Spec.lang_monoid_laws stlc_spec stlc_val :=
+  {| Spec.v_sub_proper := @v_sub_eq ;
+     Spec.v_sub_var := @a_comp_id_r ;
+     Spec.v_var_sub := @a_comp_id_l ;
+     Spec.v_sub_sub := @a_comp_assoc ;
+  |} .
+
+Program Definition stlc_conf_laws : @Spec.lang_module_laws stlc_spec stlc_val stlc_conf :=
+  {| Spec.c_sub_proper := @s_sub_eq ;
+     Spec.c_var_sub := @s_sub_id_l ;
+     Spec.c_sub_sub := @s_sub_sub ;
+  |} .
+
+Definition stlc_var_laws : @Spec.var_assumptions stlc_spec stlc_val .
+  econstructor; intros.
+  - unfold a_id in H; now dependent induction H.
+  - induction v; try (apply inr; intros [ i H ]; now inversion H).
+    apply inl; econstructor; auto.
+  - destruct X as [ i H ].
+    induction v; try now inversion H.
+    refine (h ,' eq_refl).
+Defined.
+
+Program Definition stlc_machine : @Spec.machine stlc_spec stlc_val stlc_conf :=
+  {| Spec.eval := @eval ;
+     Spec.app := @p_app ; |}.
+
+From Coinduction Require Import coinduction lattice rel tactics.
+From OGS.ITree Require Import ITree Eq Structure.
+From OGS.OGS Require Import Spec.
+
+Lemma stlc_machine_law : @Spec.machine_laws stlc_spec stlc_val stlc_conf stlc_machine .
+  econstructor; intros; unfold stlc_spec, stlc_val in *; cbn.
+  - intros ? ? H1; now apply p_app_eq.
+  - destruct x; dependent elimination m; cbn; f_equal.
+  - revert c e; unfold comp_eq, it_eq; coinduction R CIH; intros c e.
+    destruct c. cbn in v.
+    dependent elimination t.
+    * dependent elimination v.
+      + simpl c_sub.
+        unfold stlc_new.eval at 2.
+        cbn - [ stlc_new.eval ].
+        change (it_eqF ∅ₑ ?a ?b T1_0 (observe ?x) (_observe ?y)) with (it_eq_bt ∅ₑ a R T1_0 x y).
+        refine (gfp_bt (it_eq_map ∅ₑ _) R T1_0 _ _ _); reflexivity.
+      + cbn; econstructor.
+        exact (CIH (Cut t1 (KArg v0 v)) e).
+      + dependent elimination v0.
+        ++ simpl s_subst.
+           unfold stlc_new.eval at 2.
+           cbn - [ stlc_new.eval ].
+           change (it_eqF ∅ₑ ?a ?b T1_0 (observe ?x) (_observe ?y)) with (it_eq_bt ∅ₑ a R T1_0 x y).
+           refine (gfp_bt (it_eq_map ∅ₑ _) R T1_0 _ _ _); reflexivity.
+        ++ cbn; econstructor.
+           change (LamRec _) with (v_subst e _ (LamRec t0)) at 1.
+           rewrite t_sub2_sub.
+           exact (CIH (Cut (t0 /ₜ[ LamRec t0 , v1 ]) v2) e).
+    * cbn; econstructor.
+      exact (CIH (Cut t1 (KFun t0 v)) e).
+  - destruct u as [ a [ i [ p γ ] ]].
+    unfold nf_ty', nf_var', nf_val', a_id; cbn in *.
+    destruct a; dependent elimination p; cbn in *.
+    all: unfold comp_eq; apply it_eq_unstep; cbn; econstructor.
+    all: do 3 (unshelve econstructor; auto; cbn).
+    all: intros ? h; do 3 (dependent elimination h; auto).
+  - intros [ x p ].
+    destruct x; dependent elimination p; econstructor.
+    * intros [ z p ] H.
+      destruct z; dependent elimination p; dependent elimination H.
+      + dependent elimination v; try now destruct (p (_ ,' eq_refl)).
+        apply it_eq_step in i0; now inversion i0.
+      + dependent elimination v; try now destruct (p (_ ,' eq_refl)).
+        apply it_eq_step in i0; now inversion i0.
+    * intros [ z p ] H.
+      destruct z; dependent elimination p; dependent elimination H.
+      + cbn in *.
+        pose (vv :=e (t+ a) Ctx.top); change (e (t+ a) Ctx.top) with vv in i0; remember vv; clear vv Heqv0 e.
+        dependent elimination v; try now destruct (p (_ ,' eq_refl)).
+        apply it_eq_step in i0; now inversion i0.
+        dependent elimination v0; apply it_eq_step in i0; cbn in i0; dependent elimination i0.
+        unfold msg_of_nf' in r_rel; cbn in r_rel.
+        inversion_sigma r_rel; dependent elimination r_rel1; clear .
+        econstructor; intros [ z p ] H.
+        destruct z; dependent elimination p; dependent elimination H.
+        ++ dependent elimination v; try now destruct (p (_ ,' eq_refl)).
+           apply it_eq_step in i0; now inversion i0.
+        ++ dependent elimination v; try now destruct (p (_ ,' eq_refl)).
+           apply it_eq_step in i0; now inversion i0.
+      + cbn in *.
+        pose (vv :=e (t+ a) Ctx.top); change (e (t+ a) Ctx.top) with vv in i0; remember vv; clear vv Heqv0 e.
+        dependent elimination v; try now destruct (p (_ ,' eq_refl)).
+        apply it_eq_step in i0; now inversion i0.
+        dependent elimination v0; apply it_eq_step in i0; cbn in i0; dependent elimination i0.
+        unfold msg_of_nf' in r_rel; cbn in r_rel.
+        inversion_sigma r_rel; inversion r_rel1.
+Qed.
+
+Check (@Spec.inj_init_act stlc_spec stlc_val stlc_conf).
+
+Definition interp_act_s Δ {Γ} (c : state Γ) : @ogs_act stlc_spec Δ (∅ ▶ Γ) :=
+  @Spec.m_strat stlc_spec stlc_val stlc_conf stlc_machine Δ (∅ ▶ Γ)
+    (@Spec.inj_init_act stlc_spec stlc_val stlc_conf Δ Γ c) .
+Notation "⟦ t ⟧ₛ" := (interp_act_s _ t) .
+
+Definition ogs_weq_act Δ {Γ} : relation (@ogs_act stlc_spec Δ (∅ ▶ Γ)) := fun u v => u ≈ v .
+Notation "u ≈[ogs Δ ]≈ v" := (ogs_weq_act Δ u v) (at level 40).
+
+Definition stlc_eval_to_msg {Γ : t_ctx} : state Γ -> delay (@msg' stlc_spec Γ) :=
+  @eval_to_msg stlc_spec stlc_val stlc_conf stlc_machine Γ .
+
+Definition subst_eq Δ {Γ} : relation (state Γ) :=
+  fun u v => forall (σ : Γ =[stlc_new.val]> Δ), stlc_eval_to_msg (s_subst σ u) ≈ stlc_eval_to_msg (s_subst σ v) .
+Notation "x ≈[sub Δ ]≈ y" := (subst_eq Δ x y) (at level 10).
+
+Theorem stlc_subst_correct Δ {Γ} (x y : state Γ)
+  : ⟦ x ⟧ₛ ≈[ogs Δ ]≈ ⟦ y ⟧ₛ -> x ≈[sub Δ ]≈ y .
+  exact (@ogs_correction stlc_spec stlc_val stlc_val_laws stlc_conf stlc_conf_laws stlc_var_laws
+           stlc_machine stlc_machine_law Γ Δ x y).
+Qed.
+
+Definition c_of_t_p {Γ x} (t : term Γ (t+ x)) : state (Γ ▶ t- x) :=
+  Cut (t_shift _ t) (Var Ctx.top) .
+Notation "⟦ t ⟧ₚ" := (⟦ c_of_t_p t ⟧ₛ) .
+
+Definition a_of_sk_p {Γ Δ x} (s : Γ =[stlc_new.val]> Δ) (k : stlc_new.val Δ (t- x))
+  : (Γ ▶ t- x) =[stlc_new.val]> Δ :=
+  s_append s k .
+
+Definition ciu_p_eq Δ {Γ x} : relation (term Γ (t+ x)) :=
+  fun u v => forall (σ : Γ =[stlc_new.val]> Δ) (k : stlc_new.val Δ (t- x)),
+      stlc_eval_to_msg (Cut (t_subst σ _ u) k) ≈ stlc_eval_to_msg (Cut (t_subst σ _ v) k) .
+Notation "x ≈[ciu Δ ]≈ y" := (ciu_p_eq Δ x y) (at level 10).
+
+Lemma sub_csk_p {Γ Δ x} (t : term Γ (t+ x)) (s : Γ =[stlc_new.val]> Δ) (k : stlc_new.val Δ (t- x))
+              : Cut (t_subst s _ t) k = s_subst (a_of_sk_p s k) (c_of_t_p t) .
+  cbn; f_equal; unfold t_shift; now rewrite t_sub_ren.
+Qed.
+
+Theorem mu_ciu_p_correct Δ {Γ t} (x y : term Γ (t+ t)) : ⟦ x ⟧ₚ ≈[ogs Δ ]≈ ⟦ y ⟧ₚ -> x ≈[ciu Δ ]≈ y .
+  intros H σ k.
+  rewrite 2 sub_csk_p.
+  now apply stlc_subst_correct.
+Qed.
